Cleaning, there is still much more cleaning to do, but enough for the time being.

Loop/Lemmas.lean
@@ -24,38 +24,34 @@ theorem inc_value_nil_succ : inc_value [] (n + 1) = 0 :: inc_value [] n := rfl
 theorem inc_value_cons_zero : inc_value (x :: xs) 0 = (x + 1) :: xs := rfl
 theorem inc_value_cons_succ : inc_value (x :: xs) (n + 1) = x :: inc_value xs n := rfl
 
-theorem concat_is_seq_execution {p p' : Program} : p ++ p' = seq_execution p p' := by rfl
+theorem concat_eq_seq_execution {p p' : Program} : p ++ p' = seq_execution p p' := rfl
 
-theorem seq_execution_unfold : execution_from_state xs (seq_execution p p') = execution_from_state (execution_from_state xs p) p' := by simp [execution_from_state]
+theorem seq_execution_unfold : execution_from_state xs (seq_execution p p')
+  = execution_from_state (execution_from_state xs p) p' := by simp only [execution_from_state]
 
-theorem zeros_succ : List.zeros (n + 1) = 0 :: List.zeros n := by
-  simp [List.zeros, List.replicate]
+theorem List.zeros_zero : List.zeros 0 = [] := rfl
 
-theorem zeros_length : (List.zeros n).length = n := by
+theorem List.zeros_succ : List.zeros (n + 1) = 0 :: List.zeros n := by
+  simp only [List.zeros, List.replicate]
+
+theorem List.zeros_length : (List.zeros n).length = n := by
   dsimp [List.zeros]
   rw [List.length_replicate]
 
-theorem value_at_zeros_is_zero (n k : Nat) : value_at (List.zeros n) k = 0 := by
+theorem value_at_zeros_eq_zero (n k : Nat) : value_at (List.zeros n) k = 0 := by
   revert n
   induction k
-  case zero =>
-    intro n
-    cases n <;> simp [value_at]
-  case succ ih =>
-    intro n
-    cases n
-    · simp [value_at]
-    · simp [zeros_succ, value_at_cons_succ, ih]
+  all_goals intro n; cases n <;> simp only [List.zeros_zero, List.zeros_succ, value_at_nil,
+    value_at_cons_zero, value_at_cons_succ, *]
 
 theorem append_zeros_does_not_change_value_at (xs : VarState) (n k : Nat) :
     value_at xs k = value_at (xs ++ List.zeros n) k := by
   revert k
   induction xs
-  case nil => simp [value_at_nil, value_at_zeros_is_zero]
-  case cons head tail tail_ih =>
+  case nil => simp [value_at_nil, value_at_zeros_eq_zero]
+  case cons _ tail tail_ih =>
     intro k
-    cases k
-    all_goals simp [value_at_cons_zero, value_at_cons_succ, tail_ih]
+    cases k <;> simp [value_at_cons_zero, value_at_cons_succ, tail_ih]
 
 theorem clear_value_clears_value (xs : VarState) :
     value_at (clear_value xs n) k = if (n = k) then 0 else value_at xs k := by
@@ -66,9 +62,9 @@ theorem clear_value_clears_value (xs : VarState) :
   case cons x xs xs_ih =>
     intro n k
     cases n
-    · cases k <;> simp [clear_value, value_at]
+    · cases k <;> dsimp [clear_value, value_at]
     · cases k
-      · simp [clear_value, value_at]
+      · dsimp [clear_value, value_at]
       · simp [value_at_cons_succ]
         exact xs_ih
 
@@ -80,90 +76,83 @@ theorem inc_value_increments_value (xs : VarState) :
     intro n
     induction n
     case zero =>
-      simp [inc_value_nil_zero, value_at_nil]
+      dsimp [inc_value_nil_zero, value_at_nil]
       intro k
-      cases k <;> simp [value_at]
-    case succ n n_ih =>
-      simp [inc_value, value_at_nil]
+      cases k <;> dsimp [value_at]
+    case succ _ n_ih =>
+      dsimp [inc_value, value_at_nil]
       intro k
       cases k
-      · simp [value_at_cons_zero]
+      · dsimp [value_at_cons_zero]
       · simp [value_at_cons_succ]
-        simp [value_at_nil] at n_ih
+        dsimp [value_at_nil] at n_ih
         exact n_ih
   case cons x xs xs_ih =>
     intro n
     cases n
-    · simp [inc_value_cons_zero, value_at_cons_succ]
+    · dsimp [inc_value_cons_zero, value_at_cons_succ]
       intro k
-      cases k <;> simp [value_at]
+      cases k <;> dsimp [value_at]
     · simp [inc_value_cons_succ]
       intro k
       cases k <;> simp [value_at_cons_zero, value_at_cons_succ, xs_ih]
 
 theorem loop_inc_adds_value :
     execution_from_state (x :: xs) (LOOP X n DO INC X 0 END) = (x + value_at (x :: xs) n) :: xs := by
-  simp [execution_from_state]
+  simp only [execution_from_state]
   generalize value_at (x :: xs) n = k
   revert x
   induction k
-  case zero =>
-    simp [loop_n_times]
-  case succ k k_ih =>
-    simp_arith [loop_n_times, execution_from_state, inc_value, k_ih]
+  all_goals simp_arith [loop_n_times, execution_from_state, inc_value, *]
 
 theorem same_values_same_execution (p : Program) (xs ys : VarState) :
-    (∀ k : Nat, value_at xs k = value_at ys k) → ∀ k : Nat, value_at (execution_from_state xs p) k = value_at (execution_from_state ys p) k := by
+    (∀ k : Nat, value_at xs k = value_at ys k) → ∀ k : Nat, value_at (execution_from_state xs p) k
+      = value_at (execution_from_state ys p) k := by
   revert xs ys
   induction p
   case clear_var n =>
-    intro xs ys h
-    simp [execution_from_state, clear_value_clears_value, h]
+    intro xs ys h _
+    simp only [execution_from_state, clear_value_clears_value, h]
   case increment_var n =>
-    intro xs ys h
-    simp [execution_from_state, inc_value_increments_value, h]
+    intro xs ys h _
+    simp only [execution_from_state, inc_value_increments_value, h]
   case loop_var n inner inner_ih =>
     intro xs ys h
-    simp [execution_from_state, h]
+    simp only [execution_from_state, h]
     generalize value_at ys n = x
     revert xs ys
     induction x
     case zero =>
-      intro xs ys h
+      intro _ _ h
       simp [loop_n_times, h]
-    case succ x x_ih =>
+    case succ _ x_ih =>
       intro xs ys h
-      simp [loop_n_times]
+      simp only [loop_n_times]
       apply x_ih (execution_from_state xs inner) (execution_from_state ys inner)
       exact inner_ih xs ys h
-  case seq_execution p p' p_ih p'_ih =>
-    intro xs ys h
-    simp [execution_from_state]
+  case seq_execution _ _ p_ih p'_ih =>
+    intros
+    simp only [execution_from_state]
     apply p'_ih
     apply p_ih
-    exact h
+    assumption
 
 theorem append_zeros_does_not_change_execution (n k : Nat) :
-    value_at (execution_from_state (xs ++ List.zeros n) p) k = value_at (execution_from_state xs p) k := by
-  have := append_zeros_does_not_change_value_at xs n
-  have := same_values_same_execution p xs (xs ++ List.zeros n) this k
-  exact this.symm
+     value_at (execution_from_state xs p) k = value_at (execution_from_state (xs ++ List.zeros n) p) k:=
+  same_values_same_execution p xs (xs ++ List.zeros n) (append_zeros_does_not_change_value_at xs n) k
 
 theorem clear_value_clears_succ_largest_index (xs : VarState) (l_h : xs.length ≥ k + 1) :
     clear_value (xs ++ ys) k = (clear_value xs k) ++ ys := by
   revert k
   induction xs
   case nil =>
-    intro k h
-    absurd h
-    exact Nat.not_succ_le_zero k
-  case cons x xs xs_ih =>
+    intros
+    contradiction
+  case cons _ _ xs_ih =>
     intro k
     cases k
-    case zero =>
-      simp [clear_value]
-    case succ k =>
-      simp [clear_value_cons_succ]
+    · simp [clear_value]
+    · simp [clear_value_cons_succ]
       exact xs_ih
 
 theorem inc_value_increments_succ_largest_index (xs : VarState) (l_h : xs.length ≥ k + 1) :
@@ -171,16 +160,13 @@ theorem inc_value_increments_succ_largest_index (xs : VarState) (l_h : xs.length
   revert k
   induction xs
   case nil =>
-    intro k h
-    absurd h
-    exact Nat.not_succ_le_zero k
-  case cons x xs xs_ih =>
+    intros
+    contradiction
+  case cons _ _ xs_ih =>
       intro k
       cases k
-      case zero =>
-        simp [inc_value]
-      case succ k =>
-        simp [inc_value_cons_succ]
+      · simp [inc_value]
+      · simp [inc_value_cons_succ]
         exact xs_ih
 
 theorem value_at_first_k (v : VectNat n) (n_h : n > k) :
@@ -188,35 +174,25 @@ theorem value_at_first_k (v : VectNat n) (n_h : n > k) :
   revert k
   induction n
   case zero =>
-    intro k k_h
-    absurd k_h
-    have : ¬0 > k := by simp
-    exact this
-  case succ n n_ih =>
+    intros
+    contradiction
+  case succ _ n_ih =>
     let ⟨ys, ys_l⟩ := v
     simp
     cases ys
     case nil =>
       intros
-      have : ¬0 ≥ 1 := by simp
-      absurd this
-      have : 0 ≥ 1 := by calc
-        0 = n + 1 := ys_l
-        _ ≥ 1 := by simp
-      exact this
-    case cons y ys =>
+      contradiction
+    case cons _ ys =>
       intro k k_h
-      have tail_l : ys.length = n := by
-        rw [List.length] at ys_l
-        exact Nat.succ_injective ys_l
       cases k
       case zero =>
-        simp [value_at_cons_zero]
+        dsimp [value_at_cons_zero]
       case succ k =>
         simp [value_at_cons_succ]
-        have : k < n := Nat.lt_of_succ_lt_succ k_h
-        have := n_ih ⟨ys, tail_l⟩ this
-        simp at this
+        rewrite [List.length, Nat.succ_inj] at ys_l
+        have := n_ih ⟨ys, ys_l⟩ (Nat.lt_of_succ_lt_succ k_h)
+        dsimp at this
         assumption
 
 theorem execution_from_state_long_enough_preserves_length (p : Program) (v : VectNat n) (n_h : n ≥ highest_var p + 1) :
@@ -227,139 +203,122 @@ theorem execution_from_state_long_enough_preserves_length (p : Program) (v : Vec
     induction k
     case zero =>
       intro n v n_h
-      simp [highest_var] at n_h
+      dsimp [highest_var] at n_h
       cases n
       case zero =>
-        absurd n_h
-        have : ¬1 ≤ 0 := by simp
-        exact this
+        contradiction
       case succ n =>
         let ⟨x :: xs, xs_l⟩ := v
         simp at xs_l
         simp [execution_from_state, clear_value, xs_l]
     case succ k k_ih =>
       intro n v n_h
-      simp [highest_var] at n_h
+      dsimp [highest_var] at n_h
       cases n
       case zero =>
-        have : 1 ≤ 0 := by
-          have : 1 ≤ k + 1 + 1 := by simp
-          exact Nat.le_trans this n_h
-        absurd this
-        have : ¬1 ≤ 0 := by simp
-        exact this
+        contradiction
       case succ n =>
         simp at n_h
         let ⟨x :: xs, xs_l⟩ := v
         simp [execution_from_state, clear_value_cons_succ]
         simp at xs_l
         have := k_ih ⟨xs, xs_l⟩ n_h
-        simp [execution_from_state] at this
+        simp only [execution_from_state] at this
         assumption
 
   case increment_var k =>
     induction k
     case zero =>
       intro n v n_h
-      simp [highest_var] at n_h
+      dsimp [highest_var] at n_h
       cases n
       case zero =>
-        absurd n_h
-        have : ¬1 ≤ 0 := by simp
-        exact this
+        contradiction
       case succ n =>
         let ⟨x :: xs, xs_l⟩ := v
         simp at xs_l
         simp [execution_from_state, inc_value, xs_l]
     case succ k k_ih =>
       intro n v n_h
-      simp [highest_var] at n_h
+      dsimp [highest_var] at n_h
       cases n
       case zero =>
-        have : 1 ≤ 0 := by
-          have : 1 ≤ k + 1 + 1 := by simp
-          exact Nat.le_trans this n_h
-        absurd this
-        have : ¬1 ≤ 0 := by simp
-        exact this
+        contradiction
       case succ n =>
         simp at n_h
         let ⟨x :: xs, xs_l⟩ := v
         simp [execution_from_state, inc_value_cons_succ]
         simp at xs_l
         have := k_ih ⟨xs, xs_l⟩ n_h
-        simp [execution_from_state] at this
+        simp only [execution_from_state] at this
         assumption
 
   case loop_var k inner inner_ih =>
-    simp [execution_from_state]
+    simp only [execution_from_state]
     intro n v
     generalize value_at v.toList k = m
     revert n v
     induction m
     case zero =>
       simp [loop_n_times]
-    case succ m m_ih =>
+    case succ _ m_ih =>
       intro n v n_h
-      simp [loop_n_times]
+      simp only [loop_n_times]
       let ys := execution_from_state v.toList inner
-      simp [highest_var] at n_h
-      have ineq : highest_var inner + 1 ≤ n := by
+      dsimp [highest_var] at n_h
+      have : highest_var inner + 1 ≤ n := by
         have : highest_var inner + 1 ≤ max k (highest_var inner) + 1 := by simp
         exact Nat.le_trans this n_h
-      have := inner_ih v ineq
-      let w' : VectNat n := ⟨ys, this⟩
+      let w' : VectNat n := ⟨ys, inner_ih v this⟩
       have : execution_from_state v.toList inner = w'.toList := rfl
-      rw [this]
+      rewrite [this]
       exact m_ih w' n_h
 
   case seq_execution p p' p_ih p'_ih =>
     intro n v n_h
     let ys := execution_from_state v.toList p
     have : n ≥ highest_var p + 1 := by
-      rw [highest_var] at n_h
+      rewrite [highest_var] at n_h
       have : max (highest_var p) (highest_var p') + 1 ≥ highest_var p + 1 := by simp
       exact Nat.le_trans this n_h
-    have := p_ih v this
-    let w' : VectNat n := ⟨ys, this⟩
-    simp [execution_from_state]
+    let w' : VectNat n := ⟨ys, p_ih v this⟩
+    simp only [execution_from_state]
     have : execution_from_state v.toList p = w'.toList := rfl
-    rw [this]
+    rewrite [this]
     have : n ≥ highest_var p' + 1 := by
-      rw [highest_var] at n_h
+      rewrite [highest_var] at n_h
       have : max (highest_var p) (highest_var p') + 1 ≥ highest_var p' + 1 := by simp
       exact Nat.le_trans this n_h
     exact p'_ih w' this
 
-theorem execution_from_state_gt_highest_append {n : Nat} (v : VectNat (n + 1)) (n_h : n ≥ highest_var p) :
+-- Maybe remove this
+theorem execution_from_state_gt_highest_append_vector {n : Nat} (v : VectNat (n + 1)) (n_h : n ≥ highest_var p) :
     execution_from_state (v.toList ++ xs) p = (execution_from_state v.toList p) ++ xs := by
   revert n
   induction p
   case clear_var k =>
     intro n v n_h
-    simp [execution_from_state]
+    simp only [execution_from_state]
     have : v.toList.length ≥ k + 1 := by
-      have : k ≤ n := by simp [highest_var] at n_h; assumption
-      simp_arith [this]
+      have : k ≤ n := by dsimp [highest_var] at n_h; assumption
+      simp [this]
     exact clear_value_clears_succ_largest_index v.toList this
-    -- have := clear_value_clears_succ_largest_index v.toList
   case increment_var k =>
     intro n v n_h
-    simp [execution_from_state]
+    simp only [execution_from_state]
     have : v.toList.length ≥ k + 1 := by
-      have : k ≤ n := by simp [highest_var] at n_h; assumption
-      simp_arith [this]
+      have : k ≤ n := by dsimp [highest_var] at n_h; assumption
+      simp [this]
     exact inc_value_increments_succ_largest_index v.toList this
   case loop_var k inner inner_ih =>
     intro n v n_h
-    simp [execution_from_state]
+    simp only [execution_from_state]
     have : value_at (v.toList ++ xs) k = value_at v.toList k := by
       have : n ≥ k := by
-        simp [highest_var] at n_h
-        exact n_h.left
-      have : n + 1 > k := by simp_arith [this]
-      exact value_at_first_k v this
-    rw [this]
+        dsimp [highest_var] at n_h
+        exact Nat.le_trans (Nat.le_max_left _ _) n_h
+      exact value_at_first_k v (Nat.lt_succ_of_le this)
+    rewrite [this]
     generalize value_at v.toList k = m
     revert v n
     induction m
@@ -370,57 +329,67 @@ theorem execution_from_state_gt_highest_append {n : Nat} (v : VectNat (n + 1)) (
       intro n v n_h _
       simp [loop_n_times]
       have : n ≥ highest_var inner := by
-        simp [highest_var] at n_h
-        exact n_h.right
-      simp[inner_ih v this]
+        dsimp [highest_var] at n_h
+        exact Nat.le_trans (Nat.le_max_right _ _) n_h
+      rewrite [inner_ih v this]
       let ys := execution_from_state v.toList inner
-      have : ys.length = n + 1 := by
-        have : n + 1 ≥ highest_var inner + 1 := by simp_arith [this]
-        simp [execution_from_state_long_enough_preserves_length inner v this]
+      have : ys.length = n + 1 := execution_from_state_long_enough_preserves_length inner v (Nat.add_le_add_right this 1)
       let v' : VectNat (n + 1) := ⟨ys, this⟩
       have : execution_from_state v.toList inner = v'.toList := rfl
-      rw [this]
+      rewrite [this]
       have : value_at (v'.toList ++ xs) k = value_at v'.toList k := by
         have : n ≥ k := by
-          simp [highest_var] at n_h
-          exact n_h.left
-        have : n + 1 > k := by simp_arith [this]
-        exact value_at_first_k v' this
+          dsimp [highest_var] at n_h
+          exact Nat.le_trans (Nat.le_max_left _ _) n_h
+        exact value_at_first_k v' (Nat.lt_succ_of_le this)
       exact m_ih v' n_h this
 
   case seq_execution p p' p_ih p'_ih =>
     intro n v n_h
-    simp [execution_from_state]
+    simp only [execution_from_state]
     have : n ≥ highest_var p := by
-      simp [highest_var] at n_h
-      exact n_h.left
-    rw [p_ih v this]
+        dsimp [highest_var] at n_h
+        exact Nat.le_trans (Nat.le_max_left _ _) n_h
+    rewrite [p_ih v this]
     let ys := execution_from_state v.toList p
-    have : ys.length = n + 1 := by
-      have : n + 1 ≥ highest_var p + 1 := by simp [this]
-      simp [execution_from_state_long_enough_preserves_length p v this]
+    have : ys.length = n + 1 := execution_from_state_long_enough_preserves_length p v (Nat.add_le_add_right this 1)
     let v' : VectNat (n + 1) := ⟨ys, this⟩
     have : execution_from_state v.toList p = v'.toList := rfl
-    rw [this]
+    rewrite [this]
     have : n ≥ highest_var p' := by
-      simp [highest_var] at n_h
-      exact n_h.right
+      dsimp [highest_var] at n_h
+      exact Nat.le_trans (Nat.le_max_right _ _) n_h
     exact p'_ih v' this
 
+theorem execution_from_state_gt_highest_append_list {xs : VarState} (n_h : xs.length ≥ highest_var p + 1) :
+    execution_from_state (xs ++ ys) p = (execution_from_state xs p) ++ ys := by
+  have := calc
+    1 ≤ highest_var p + 1 := by simp_arith
+    _ ≤ xs.length := n_h
+  have xs_l' := (Nat.sub_add_cancel this).symm
+  have : List.length xs - 1 ≥ highest_var p := by
+    have := Nat.sub_le_sub_right n_h 1
+    rewrite [Nat.add_sub_cancel] at this
+    assumption
+  have := @execution_from_state_gt_highest_append_vector p ys (xs.length - 1) ⟨xs, xs_l'⟩ this
+  dsimp at this
+  assumption
+
+
 theorem execution_from_init_state_ge_highest_append (v : VectNat n) (n_h : n ≥ highest_var p) :
-    execution_from_state (init_state v ++ xs) p = (execution_from_state (init_state v) p) ++ xs := by
-  apply execution_from_state_gt_highest_append (0 ::ᵥ v) n_h
+    execution_from_state (init_state v ++ xs) p = (execution_from_state (init_state v) p) ++ xs :=
+  execution_from_state_gt_highest_append_vector (0 ::ᵥ v) n_h
 
 theorem execution_from_state_append_xs (v : VectNat n) :
     execution_from_state (init_state v ++ List.zeros (highest_var p - n) ++ xs) p
     = (execution_from_state (init_state v ++ List.zeros (highest_var p - n)) p) ++ xs := by
-  rw [init_state]
+  rewrite [init_state]
   let ys := v.toList ++ List.zeros (highest_var p - n)
   let m := ys.length
   have m_h : m ≥ highest_var p := by
     simp [m, ys]
-    rw [Nat.add_comm, Nat.sub_add_eq_max]
-    exact Nat.le_max_left (highest_var p) n
+    rewrite [Nat.add_comm, Nat.sub_add_eq_max]
+    exact Nat.le_max_left _ _
   let w : VectNat m := ⟨ys, rfl⟩
   have : 0 :: w.toList = 0 :: v.toList ++ List.zeros (highest_var p - n) := rfl
   rw [←this, ←init_state, execution_from_init_state_ge_highest_append w m_h]
@@ -446,7 +415,7 @@ theorem cleanly_computable_append_zeros_append_xs {f : VectNat n → Nat} {k : N
   intro xs v k_h
   have : (highest_var p - n) + (k - (highest_var p - n)) = k := by
     have := Nat.sub_add_eq_max k (highest_var p - n)
-    rw [Nat.add_comm, Nat.max_eq_left k_h] at this
+    rewrite [Nat.add_comm, Nat.max_eq_left k_h] at this
     assumption
   let m := highest_var p - n
 
@@ -463,7 +432,7 @@ theorem cleanly_computable_append_zeros_append_xs {f : VectNat n → Nat} {k : N
     _ =
     f v :: v.toList ++ List.zeros k ++ xs := by rw [append_zeros_addition _ _ _ this]
 
-theorem highest_var_concat : highest_var (p1 ++ p2) = max (highest_var p1) (highest_var p2) := by simp [highest_var]
+theorem highest_var_concat : highest_var (p1 ++ p2) = max (highest_var p1) (highest_var p2) := by dsimp [highest_var]
 
 theorem loop_n_times_loop : loop_n_times (n + 1) xs p = execution_from_state (loop_n_times n xs p) p := by
   revert xs
@@ -472,7 +441,7 @@ theorem loop_n_times_loop : loop_n_times (n + 1) xs p = execution_from_state (lo
     simp [loop_n_times]
   case succ n n_ih =>
     intro xs
-    have : loop_n_times ((n + 1) + 1) xs p = loop_n_times (n + 1) (execution_from_state xs p) p := by simp [loop_n_times]
+    have : loop_n_times ((n + 1) + 1) xs p = loop_n_times (n + 1) (execution_from_state xs p) p := by simp only [loop_n_times]
     rw [this, n_ih, ←loop_n_times]
 
 theorem value_at_n : (xs.length = n) →
@@ -481,7 +450,7 @@ theorem value_at_n : (xs.length = n) →
   induction n
   case zero =>
     simp [value_at_cons_zero]
-  case succ n n_ih =>
+  case succ _ n_ih =>
     intro xs xs_l
     let (x :: xs) := xs
     simp at xs_l
@@ -494,7 +463,7 @@ theorem clear_value_at_n : (xs.length = n) →
   induction n
   case zero =>
     simp [clear_value]
-  case succ n n_ih =>
+  case succ _ n_ih =>
     intro xs xs_l
     let (x :: xs) := xs
     simp at xs_l
@@ -506,7 +475,7 @@ theorem inc_value_at_n : (xs.length = n) →
   induction n
   case zero =>
     simp [inc_value]
-  case succ n n_ih =>
+  case succ _ n_ih =>
     intro xs xs_l
     let (x :: xs) := xs
     simp at xs_l
@@ -525,17 +494,17 @@ theorem inc_X_i_X_j_adds_value : (xs.length = n) →
     simp [loop_n_times]
   case succ k k_ih =>
     rewrite [loop_n_times_loop, k_ih]
-    simp [execution_from_state]
+    simp only [execution_from_state]
     rw [inc_value_at_n xs_l, Nat.add_assoc y k 1]
 
 theorem nested_max_lemma {a b : Nat} :
     max (max a b) (max (a + 1) (b + 1)) = max (a + 1) (b + 1) := by
   cases Nat.decLe a b
   case isTrue h =>
-    repeat rw [Nat.max_def]
+    repeat rewrite [Nat.max_def]
     simp [h]
   case isFalse h =>
-    repeat rw [Nat.max_def]
+    repeat rewrite [Nat.max_def]
     simp [h]
 
 theorem List.take_n_concat_last_eq (xs : List α) (xs_l : xs.length = n + 1) :
@@ -543,76 +512,92 @@ theorem List.take_n_concat_last_eq (xs : List α) (xs_l : xs.length = n + 1) :
   revert xs
   induction n
   case zero =>
-    intro xs xs_l
+    intro xs _
     let [x] := xs
     dsimp [List.take]
   case succ n n_ih =>
     intro xs xs_l
     let (x :: xs) := xs
-    simp_arith [List.length] at xs_l
+    simp at xs_l
     dsimp [List.take]
     rewrite [List.cons_inj_right, List.getLast_cons (List.ne_nil_of_length_eq_add_one xs_l)]
     exact n_ih xs xs_l
 
+  def cons_last_construction (v : Mathlib.Vector α (n + 1)) :
+      (t : α) ×' (xs : List α) ×' (xs.length = n) ×' (v.toList = xs ++ [t]) :=
+    let t := v.toList.getLast (List.ne_nil_of_length_eq_add_one v.length_val)
+    let xs := v.toList.take n
+    let v_list : v.toList = xs ++ [t] := List.take_n_concat_last_eq v.toList (v.length_val)
+    let xs_l : xs.length = n := by
+      have := congrArg (List.length) v_list
+      simp [List.length_append] at this
+      exact this.symm
+    ⟨t, xs, xs_l, v_list⟩
+
+
 theorem List.zeros_concat : List.zeros (n + 1) = List.zeros n ++ [0] := by
-  have := take_n_concat_last_eq (zeros (n + 1)) zeros_length
+  have := take_n_concat_last_eq (zeros (n + 1)) List.zeros_length
   simp at this
   rewrite [←List.zeros] at this
   assumption
 
+-- Note: attempting to use the simplifier does not work. Why?
+theorem max_le_lemma {a b c d : Nat} (h_1 : a ≤ c) (h_2 : b ≤ d) : max a b ≤ max c d := by
+  have h_3 := Nat.le_trans h_1 (Nat.le_max_left c d)
+  have h_4 := Nat.le_trans h_2 (Nat.le_max_right c d)
+  exact Nat.max_le.mpr (And.intro h_3 h_4)
+
 theorem highest_var_store : highest_var (store_X_1_to_X_succ_n idx n) = max (n + 1) (idx + n) := by
   induction n
   case zero =>
-    simp [store_X_1_to_X_succ_n, highest_var]
+    dsimp [store_X_1_to_X_succ_n, highest_var]
   case succ n n_ih =>
-    simp [store_X_1_to_X_succ_n, highest_var, n_ih]
-    rw [Nat.add_assoc n 1 1, ←Nat.add_assoc idx n 1]
+    dsimp [store_X_1_to_X_succ_n, highest_var]
+    rewrite [n_ih, ←Nat.add_assoc idx n 1]
+    rw [Nat.max_eq_right (max_le_lemma (Nat.le_succ (n + 1)) (Nat.le_succ (idx + n)))]
 
 theorem highest_var_clear : highest_var (clear_X_j_to_X_n_plus_j j n) = n + j := by
   induction n
   case zero =>
-    simp [clear_X_j_to_X_n_plus_j, highest_var]
+    dsimp [clear_X_j_to_X_n_plus_j, highest_var]
+    exact (Nat.zero_add j).symm
   case succ n n_ih =>
-    simp [clear_X_j_to_X_n_plus_j, highest_var, n_ih]
+    dsimp [clear_X_j_to_X_n_plus_j, highest_var]
+    have : n + 1 + j = n + j + 1 := by simp_arith
+    rw [n_ih, this, Nat.max_eq_right (Nat.le_succ (n + j))]
 
 theorem highest_var_setup : highest_var (setup_X_j_to_X_n_plus_j idx j n) = max (n + j) (idx + n + 1) := by
   induction n
   case zero =>
-    simp [setup_X_j_to_X_n_plus_j, highest_var]
-    rw [Nat.max_comm]
+    dsimp [setup_X_j_to_X_n_plus_j, highest_var]
+    rw [Nat.zero_add, Nat.max_comm]
   case succ n n_ih =>
-    simp [setup_X_j_to_X_n_plus_j, highest_var, n_ih]
-    have : n + 1 + j = n + j + 1 := by rw [Nat.add_assoc, Nat.add_comm 1, Nat.add_assoc]
-    rw [this]
-    have : idx + (n + 1) + 1 = idx + n + 2 := by repeat rw [Nat.add_assoc]
-    rw [this]
-    have : idx + n + 2 = (idx + n + 1) + 1 := by repeat rw [Nat.add_assoc]
-    rw [this]
-    generalize n + j = a
-    generalize idx + n + 1 = b
-    rw [Nat.max_comm (b + 1)]
-    exact nested_max_lemma
+    dsimp [setup_X_j_to_X_n_plus_j, highest_var]
+    rewrite [n_ih, Nat.max_comm (n + j)]
+    have : n + 1 + j = n + j + 1 := by simp_arith
+    rewrite [this, ←Nat.add_assoc]
+    rewrite [Nat.max_eq_right (max_le_lemma (Nat.le_succ (idx + n + 1)) (Nat.le_succ (n + j)))]
+    rw [Nat.max_comm]
 
 theorem highest_var_clear_Z (n : Nat) : highest_var (clear_Z_0_to_Z_n idx n) = idx + n:= by
   induction n
   case zero =>
-    simp [highest_var]
+    dsimp [highest_var]
   case succ n n_ih =>
-    simp  [highest_var, n_ih]
-    exact Nat.add_assoc _ _ _
+    dsimp [highest_var]
+    rw [n_ih, Nat.max_eq_right (Nat.le_succ (idx + n)), ←Nat.add_assoc]
 
 theorem clear_Z_succ : execution_from_state (x :: xs) (clear_Z_0_to_Z_n (k + 1) n)
     = x :: execution_from_state xs (clear_Z_0_to_Z_n k n) := by
   induction n
   case zero =>
     dsimp [clear_Z_0_to_Z_n]
-    simp [execution_from_state]
+    simp only [execution_from_state]
     rw [clear_value_cons_succ]
   case succ n n_ih =>
-    dsimp [clear_Z_0_to_Z_n, concat_is_seq_execution]
-    simp [execution_from_state]
-    rewrite [n_ih]
-    rewrite [clear_value_cons_succ]
+    dsimp [clear_Z_0_to_Z_n, concat_eq_seq_execution]
+    simp only [execution_from_state]
+    rewrite [n_ih, clear_value_cons_succ]
     rw [Nat.add_assoc, Nat.add_comm 1 n, Nat.add_assoc]
 
 theorem clear_Z_lemma (v : VectNat (n + 1)) : (xs.length = k) →
@@ -622,9 +607,7 @@ theorem clear_Z_lemma (v : VectNat (n + 1)) : (xs.length = k) →
   induction k
   case zero =>
     intro xs xs_l
-    have : xs = [] := List.eq_nil_of_length_eq_zero xs_l
-    rewrite [this]
-    simp
+    rewrite [List.eq_nil_of_length_eq_zero xs_l, List.nil_append, List.nil_append]
     revert v
     induction n
     case zero =>
@@ -632,27 +615,15 @@ theorem clear_Z_lemma (v : VectNat (n + 1)) : (xs.length = k) →
       simp [clear_Z_0_to_Z_n, execution_from_state, clear_value]
     case succ n n_ih =>
       intro v
-      dsimp [clear_Z_0_to_Z_n, concat_is_seq_execution]
+      dsimp [clear_Z_0_to_Z_n, concat_eq_seq_execution]
       simp [execution_from_state]
-      let xs := v.toList.take (n + 1)
-      have := List.ne_nil_of_length_eq_add_one v.length_val
-      let t := v.toList.getLast this
-      have v_list : v.toList = xs ++ [t] := List.take_n_concat_last_eq _ (by simp [this])
-      have xs_l : xs.length = n + 1 := by
-        have := congrArg (List.length) v_list
-        simp at this
-        exact this.symm
+      let ⟨t, xs, xs_l, v_list⟩ := cons_last_construction v
       rewrite [v_list]
-      have : highest_var (clear_Z_0_to_Z_n 0 n) = n := by simp_arith [highest_var_clear_Z]
-      have := @execution_from_state_gt_highest_append (clear_Z_0_to_Z_n 0 n) [t] n
-        ⟨xs, xs_l⟩ (by simp_arith [this])
-      dsimp at this
-      rewrite [this]
+      have : xs.length ≥ highest_var (clear_Z_0_to_Z_n 0 n) + 1 := by simp [highest_var_clear_Z, xs_l]
+      rewrite [execution_from_state_gt_highest_append_list this]
       have := n_ih ⟨xs, xs_l⟩
       dsimp at this
-      rewrite [this]
-      have : (List.zeros (n + 1)).length = n + 1 := by simp
-      rewrite [clear_value_at_n this]
+      rewrite [this, clear_value_at_n (@List.zeros_length (n + 1))]
       rw [←List.zeros_concat]
   case succ k k_ih =>
     intro xs xs_l
@@ -672,39 +643,31 @@ theorem clear_X_succ : execution_from_state (x :: xs) (clear_X_j_to_X_n_plus_j (
     simp [clear_X_j_to_X_n_plus_j, execution_from_state]
     rw [clear_value_cons_succ]
   case succ n n_ih =>
-    simp [clear_X_j_to_X_n_plus_j, concat_is_seq_execution, execution_from_state]
+    simp [clear_X_j_to_X_n_plus_j, concat_eq_seq_execution, execution_from_state]
     rw [n_ih, ←Nat.add_assoc, clear_value_cons_succ]
 
-theorem clear_X_lemma (v : VectNat (n + 1)) : execution_from_state v.toList (clear_X_j_to_X_n_plus_j 0 n) = List.zeros (n + 1) := by
+theorem clear_X_lemma (v : VectNat (n + 1)) : execution_from_state v.toList (clear_X_j_to_X_n_plus_j 0 n)
+    = List.zeros (n + 1) := by
   induction n
   case zero =>
     simp [clear_X_j_to_X_n_plus_j, execution_from_state, clear_value]
   case succ n n_ih =>
-    simp [clear_X_j_to_X_n_plus_j, concat_is_seq_execution, execution_from_state]
-    let xs := v.toList.take (n + 1)
-    have := List.ne_nil_of_length_eq_add_one v.length_val
-    let t := v.toList.getLast this
-    have v_list : v.toList = xs ++ [t] := List.take_n_concat_last_eq _ (by simp [this])
-    have xs_l : xs.length = n + 1 := by
-      have := congrArg (List.length) v_list
-      simp at this
-      exact this.symm
+    simp [clear_X_j_to_X_n_plus_j, concat_eq_seq_execution, execution_from_state]
+    let ⟨t, xs, xs_l, v_list⟩ := cons_last_construction v
     rewrite [v_list]
-    have : highest_var (clear_X_j_to_X_n_plus_j 0 n) ≤ n := by
+    have : highest_var (clear_X_j_to_X_n_plus_j 0 n) + 1 ≤ xs.length := by
+      rewrite [xs_l, Nat.succ_le_succ_iff]
       have : highest_var (clear_X_j_to_X_n_plus_j 0 n) = n := highest_var_clear
       rewrite [this]
       exact Nat.le_refl _
-    have := @execution_from_state_gt_highest_append (clear_X_j_to_X_n_plus_j 0 n) [t] n
-        ⟨xs, xs_l⟩ this
-    simp at this
-    rewrite [this]
+    rewrite [execution_from_state_gt_highest_append_list this]
     have := n_ih ⟨xs, xs_l⟩
-    simp at this
-    rewrite [this, clear_value_at_n]
+    dsimp at this
+    rewrite [this, clear_value_at_n (@List.zeros_length (n + 1))]
     rw [←List.zeros_concat]
-    simp
 
-theorem clear_X_1_lemma (v : VectNat (n + 1)) : execution_from_state (0 :: v.toList) (clear_X_j_to_X_n_plus_j 1 n) = 0 :: List.zeros (n + 1) := by
+theorem clear_X_1_lemma (v : VectNat (n + 1)) : execution_from_state (0 :: v.toList) (clear_X_j_to_X_n_plus_j 1 n)
+    = 0 :: List.zeros (n + 1) := by
   rw [clear_X_succ, clear_X_lemma]
 
 theorem lemma_store : ∀ c n : Nat, ∀ w : VectNat c, ∀ v : VectNat (n + 1),
@@ -717,36 +680,22 @@ theorem lemma_store : ∀ c n : Nat, ∀ w : VectNat c, ∀ v : VectNat (n + 1),
     intro c w v
     let ⟨[x], xs_l⟩ := v
     simp [Mathlib.Vector.head, store_X_1_to_X_succ_n, execution_from_state]
+    repeat rewrite [← List.cons_append]
     let ys := 0 :: x :: w.toList
-    have : 0 :: x :: (Mathlib.Vector.toList w ++ [0]) = 0 :: x :: w.toList ++ [0] := by simp
-    rewrite [this]
     have : ys.length = c + 2 := by
       dsimp [ys]
-      let ⟨ws, ws_l⟩ := w
-      dsimp
-      rw [ws_l]
+      rw [w.toList_length]
     rewrite [inc_X_i_X_j_adds_value this]
     simp [ys, value_at]
   case succ n n_ih =>
     intro c w v
-    let xs := v.toList.take (n + 1)
-    have := List.ne_nil_of_length_eq_add_one v.length_val
-    let t := v.toList.getLast this
-    have v_list : v.toList = xs ++ [t] := List.take_n_concat_last_eq _ (by simp [this])
-    rewrite [v_list]
-    have xs_l : xs.length = n + 1 := by
-      have : (xs ++ [t]).length = v.toList.length := by rw [v_list]
-      simp [List.length_concat] at this
-      assumption
-    have : 0 :: (xs ++ [t]) ++ w.toList = 0 :: xs ++ t :: w.toList := by simp
-    rewrite [this, List.zeros_concat]
-    dsimp [store_X_1_to_X_succ_n, concat_is_seq_execution]
-    simp [execution_from_state]
+    let ⟨t, xs, xs_l, v_list⟩ := cons_last_construction v
+    rewrite [v_list, ←List.cons_append, List.zeros_concat, ←List.append_assoc]
+    simp only [store_X_1_to_X_succ_n, concat_eq_seq_execution, execution_from_state]
+    rewrite [←List.append_cons _ t]
     have := calc
-          execution_from_state (0 :: (xs ++ t :: (Mathlib.Vector.toList w ++ (List.zeros (n + 1) ++ [0]))))
+          execution_from_state (0 :: xs ++ t :: Mathlib.Vector.toList w ++ List.zeros (n + 1) ++ [0])
             (store_X_1_to_X_succ_n (n + 1 + c + 2) n)
-        = execution_from_state (0 :: xs ++ t :: Mathlib.Vector.toList w ++ List.zeros (n + 1) ++ [0])
-            (store_X_1_to_X_succ_n (n + 1 + c + 2) n) := by simp
       _ = execution_from_state (0 :: xs ++ t :: Mathlib.Vector.toList w ++ List.zeros (n + 1))
             (store_X_1_to_X_succ_n (n + 1 + c + 2) n) ++ [0] := by
               have l_h : (0 :: xs ++ t :: w.toList ++ List.zeros (n + 1)).length = n + n + c + 4 := by simp_arith [xs_l]
@@ -756,34 +705,27 @@ theorem lemma_store : ∀ c n : Nat, ∀ w : VectNat c, ∀ v : VectNat (n + 1),
                 repeat rewrite [←Nat.add_assoc] at this
                 rewrite [Nat.max_eq_right this]
                 simp_arith
-              have : n + n + c + 3 ≥ highest_var (store_X_1_to_X_succ_n (n + 1 + c + 2) n) := by
-                rewrite [this]
+              have : (0 :: xs ++ t :: w.toList ++ List.zeros (n + 1)).length
+                  ≥ highest_var (store_X_1_to_X_succ_n (n + 1 + c + 2) n) + 1 := by
+                rewrite [l_h, this]
                 exact Nat.le_refl _
-              have := @execution_from_state_gt_highest_append (store_X_1_to_X_succ_n (n + 1 + c + 2) n) [0] (n + n + c + 3)
-                ⟨(0 :: xs ++ t :: w.toList ++ List.zeros (n + 1)), l_h⟩ this
-              simp at this
-              simp
-              exact this
+              rw [execution_from_state_gt_highest_append_list this]
       _ = 0 :: xs ++ t :: w.toList ++ xs ++ [0] := by
-        have := n_ih (c + 1) ⟨(t :: w.toList), by simp_arith⟩ ⟨xs, xs_l⟩
-        have := congrArg (· ++ [0]) this
-        simp at this
-        rewrite [Nat.add_comm c 1] at this
-        repeat rewrite [←Nat.add_assoc] at this
-        simp
-        assumption
-
+        have := congrArg (· ++ [0]) (n_ih (c + 1) ⟨(t :: w.toList), by simp⟩ ⟨xs, xs_l⟩)
+        dsimp at this
+        repeat rewrite [←List.cons_append] at this
+        rewrite [Nat.add_comm c 1, ←Nat.add_assoc] at this
+        rw [this]
     rewrite [this]
     have : (0 :: xs ++ t :: Mathlib.Vector.toList w ++ xs).length = n + 1 + c + 2 + n + 1 := by simp_arith [xs_l]
     rewrite [inc_X_i_X_j_adds_value this]
     have : value_at (0 :: xs ++ t :: Mathlib.Vector.toList w ++ xs ++ [0]) (n + 2) = t := by
       have : 0 :: xs ++ t :: w.toList ++ xs ++ [0] = 0 :: xs ++ t :: (w.toList ++ xs ++ [0]) := by simp
       rewrite [this]
-      have : (0 :: xs).length = n + 2 := by simp_arith [xs_l]
+      have : (0 :: xs).length = n + 2 := by simp [xs_l]
       exact value_at_n this
-    simp [this]
-    simp at this
-    assumption
+    rewrite [this]
+    simp
 
 theorem inc_X_i_X_j_succ : execution_from_state (x :: xs) (X (i + 1) += X (j + 1))
     = x :: execution_from_state xs (X i += X j) := by
@@ -796,7 +738,7 @@ theorem inc_X_i_X_j_succ : execution_from_state (x :: xs) (X (i + 1) += X (j + 1
   case succ n n_ih =>
     simp [loop_n_times_loop]
     rewrite [n_ih]
-    simp [execution_from_state]
+    simp only [execution_from_state]
     rw [inc_value_cons_succ]
 
 theorem setup_X_succ : execution_from_state (x :: xs) (setup_X_j_to_X_n_plus_j (offset + 1) (j + 1) n)
@@ -807,7 +749,7 @@ theorem setup_X_succ : execution_from_state (x :: xs) (setup_X_j_to_X_n_plus_j (
     rw [inc_X_i_X_j_succ]
   case succ n n_ih =>
     dsimp [setup_X_j_to_X_n_plus_j]
-    simp [concat_is_seq_execution, execution_from_state]
+    simp [concat_eq_seq_execution, execution_from_state]
     rewrite [n_ih, ←Nat.add_assoc]
     rewrite [inc_X_i_X_j_succ]
     simp_arith
@@ -821,62 +763,47 @@ theorem lemma_setup : ∀ c n : Nat, ∀ w : VectNat c, ∀ v : VectNat (n + 1),
   case zero =>
     intro c w v
     let ⟨[x], xs_l⟩ := v
-    simp [Mathlib.Vector.head, setup_X_j_to_X_n_plus_j]
-    have := @inc_X_i_X_j_adds_value 0 [] 0 (w.toList ++ [x]) (c + 1) rfl
-    simp at this
-    rewrite [this]
-    repeat rewrite [←List.cons_append]
+    dsimp [setup_X_j_to_X_n_plus_j]
+    have : (0 :: w.toList).length = c + 1 := by simp_all
+    rewrite [Nat.zero_add, ←List.nil_append (0 :: (w.toList ++ [x]))]
+    rewrite [inc_X_i_X_j_adds_value (by simp), ←List.cons_append]
+    simp only [List.nil_append, Nat.add_zero]
     have : (0 :: w.toList).length = c + 1 := by simp
-    rw [value_at_n this]
+    rewrite [value_at_n this]
+    simp
   case succ n n_ih =>
     intro c w v
-    let xs := v.toList.take (n + 1)
-    have := List.ne_nil_of_length_eq_add_one v.length_val
-    let t := v.toList.getLast this
-    have v_list : v.toList = xs ++ [t] := List.take_n_concat_last_eq _ (by simp [this])
-    rewrite [v_list]
-    have xs_l : xs.length = n + 1 := by
-      have : (xs ++ [t]).length = v.toList.length := by rw [v_list]
-      simp [List.length_concat] at this
-      assumption
-    simp_arith
-    dsimp [setup_X_j_to_X_n_plus_j, concat_is_seq_execution]
-    simp [execution_from_state]
-    rewrite [List.zeros_concat]
-    have := calc
-          execution_from_state ((List.zeros (n + 1) ++ [0] ++ (w.toList ++ (xs ++ [t]))))
-            (setup_X_j_to_X_n_plus_j (n + 1 + c) 0 n)
-        = execution_from_state (List.zeros (n + 1) ++ 0 :: w.toList ++ xs ++ [t])
-            (setup_X_j_to_X_n_plus_j (n + c + 1) 0 n) := by rewrite [Nat.add_comm, Nat.add_assoc, Nat.add_comm 1 (n + c)]; simp
+    let ⟨t, xs, xs_l, v_list⟩ := cons_last_construction v
+    rewrite [v_list, ←List.append_assoc, List.zeros_concat, ←List.append_cons]
+    simp only [setup_X_j_to_X_n_plus_j, concat_eq_seq_execution, execution_from_state]
 
-      _ = (execution_from_state (List.zeros (n + 1) ++ 0 :: w.toList ++ xs)
-            (setup_X_j_to_X_n_plus_j (n + c + 1) 0 n)) ++ [t] := by
-            have : highest_var (setup_X_j_to_X_n_plus_j (n + c + 1) 0 n) ≤ (2*n + c + 2) := by
-              have : highest_var (setup_X_j_to_X_n_plus_j (n + c + 1) 0 n) = (2*n + c + 2) := by rewrite [highest_var_setup] ; simp_arith
+    have := calc
+          execution_from_state (List.zeros (n + 1) ++ 0 :: w.toList ++ xs ++ [t])
+            (setup_X_j_to_X_n_plus_j (n + 1 + c) 0 n)
+        = (execution_from_state (List.zeros (n + 1) ++ 0 :: w.toList ++ xs)
+            (setup_X_j_to_X_n_plus_j (n + 1 + c) 0 n)) ++ [t] := by
+
+            have : (List.zeros (n + 1) ++ 0 :: Mathlib.Vector.toList w ++ xs).length
+                ≥ highest_var (setup_X_j_to_X_n_plus_j (n + 1 + c) 0 n) + 1 := by
+              simp_arith [xs_l]
+              have : highest_var (setup_X_j_to_X_n_plus_j (n + 1 + c) 0 n)
+                = (2*n + c + 2) := by rewrite [highest_var_setup] ; simp_arith
               rewrite [this]
               exact Nat.le_refl _
-            have := @execution_from_state_gt_highest_append (setup_X_j_to_X_n_plus_j (n + c + 1) 0 n) [t] (2*n + c + 2)
-              ⟨List.zeros (n + 1) ++ 0 :: w.toList ++ xs, by simp_arith [xs_l]⟩ this
-            simp at this
-            simp
-            rw [this]
+
+            rw [execution_from_state_gt_highest_append_list this]
       _ = xs ++ 0 :: w.toList ++ xs ++ [t] := by
         have := n_ih (c + 1) ⟨0 :: w.toList, by simp⟩ ⟨xs, xs_l⟩
-        simp_arith at this
-        rewrite [←Nat.add_assoc] at this
-        simp
-        rewrite [this]
-        simp
-
+        dsimp at this
+        rewrite [Nat.add_comm c 1, ←Nat.add_assoc] at this
+        rw [this]
     rewrite [this]
-    simp_arith
-    have := @inc_X_i_X_j_adds_value (n + 1) xs 0 (w.toList ++ xs ++ [t]) (2*n + c + 3) xs_l
-    simp at this
-    rewrite [this]
-    have := @value_at_n (2*n + c + 3) (xs ++ 0 :: w.toList ++ xs) t [] (by simp_arith [xs_l])
-    simp at this
-    rewrite [this]
-    simp
+    rewrite [List.append_assoc, List.append_assoc, List.cons_append]
+    rewrite [inc_X_i_X_j_adds_value xs_l]
+    repeat rewrite [←List.cons_append]
+    repeat rewrite [←List.append_assoc]
+    have : (xs ++ 0 :: w.toList ++ xs).length = n + 1 + c + n + 2 := by simp_arith [xs_l]
+    rw [value_at_n this, Nat.zero_add]
 
 theorem lemma_setup_X_1 : ∀ c n : Nat, ∀ w : VectNat c, ∀ v : VectNat (n + 1),
     execution_from_state (0 :: List.zeros (n + 1) ++ w.toList ++ v.toList) (setup_X_j_to_X_n_plus_j (n + c + 1) 1 n)
@@ -921,9 +848,3 @@ theorem forall_exists_function {n : Nat} (g : Fin n → VectNat m → Nat)
       suffices h : ⟨n, Nat.lt_succ_self n⟩ = i from by rewrite [h] at p_g_n_h; assumption
       suffices h : n = i.val from Fin.eq_of_val_eq h
       exact Nat.le_antisymm (Nat.ge_of_not_lt h) (Nat.le_of_lt_succ i.2)
-
--- Note: attempting to use the simplifier does not work. Why?
-theorem max_le_lemma (a b c d : Nat) (h_1 : a ≤ c) (h_2 : b ≤ d) : max a b ≤ max c d := by
-  have h_3 := Nat.le_trans h_1 (Nat.le_max_left c d)
-  have h_4 := Nat.le_trans h_2 (Nat.le_max_right c d)
-  exact Nat.max_le.mpr (And.intro h_3 h_4)
